src/provability.lean
@@ -1,0 +1,210 @@
+import lib
+
+universe u
+
+namespace classical_logic
+
+def mk' (F : Sort*) [has_negation F] [has_arrow F] [has_top F] [has_turnstile (set F) F]
+(deduction' : ∀ {T : set F} {p q : F}, T +{ p } ⊢ q → T ⊢ p ⟶ q)
+(weakening : ∀ {T : set F} {U : set F} {p : F}, T ⊆ U → T ⊢ p → U ⊢ p)
+(modus_ponens : ∀ {T : set F} {p q : F}, T ⊢ p ⟶ q → T ⊢ p → T ⊢ q)
+(by_axiom : ∀ {T : set F} {p : F}, p ∈ T → T ⊢ p)
+(imply₁ : ∀ {T : set F} {p q : F}, T ⊢ p ⟶ q ⟶ p)
+(imply₂ : ∀ {T : set F} {p q r : F}, T ⊢ (p ⟶ q ⟶ r) ⟶ (p ⟶ q) ⟶ p ⟶ r)
+(contrapose : ∀ {T : set F} {p q : F}, T ⊢ (⁻p ⟶ ⁻q) ⟶ q ⟶ p)
+(provable_top : ∀ {T : set F}, T ⊢ (⊤ : F)) : classical_logic (F : Sort*) :=
+{ deduction' := @deduction',
+  weakening := @weakening,
+  modus_ponens := @modus_ponens,
+  by_axiom := @by_axiom,
+  imply₁ := @imply₁,
+  imply₂ := @imply₂,
+  contrapose := @contrapose,
+  provable_top := @provable_top,
+  bot := ⁻⊤,
+  inf := λ p q, ⁻(p ⟶ ⁻q),
+  sup := λ p q, ⁻p ⟶ q,
+  provable_bot := by simp,  
+  and_def := by simp,
+  or_def := by simp }
+
+variables {F : Type*} (T : set F) [classical_logic F]
+
+@[simp] lemma not_top_eq_bot : (⁻⊤ : F) = ⊥ := by simp[classical_logic.provable_bot]
+
+@[simp] lemma refl (p : F) : T ⊢ p ⟶ p :=
+begin
+  have l₀ : T ⊢ (p ⟶ (p ⟶ p) ⟶ p) ⟶ (p ⟶ p ⟶ p) ⟶ p ⟶ p, simp,
+  have l₁ : T ⊢ p ⟶ (p ⟶ p) ⟶ p, simp,
+  have l₂ : T ⊢ (p ⟶ p ⟶ p) ⟶ p ⟶ p, refine modus_ponens l₀ l₁,
+  have l₃ : T ⊢ p ⟶ p ⟶ p, simp,
+  refine modus_ponens l₂ l₃
+end
+
+variables {T}
+
+@[simp] lemma insert (p) : T+{p} ⊢ p :=
+by_axiom (by simp)
+
+@[simp] lemma weakening_insert {q : F} (h : T ⊢ q) (p) : T +{ p } ⊢ q :=
+weakening (show T ⊆ T +{ p }, by { intros x h, simp[h] }) h
+
+theorem deduction {p q} : (T +{ p } ⊢ q) ↔ (T ⊢ p ⟶ q) :=
+⟨deduction', λ h, by { have : T+{p} ⊢ p ⟶ q, simp[h], exact modus_ponens this (by simp) }⟩
+
+@[simp] lemma hyp_right {p : F} (h : T ⊢ p) (q) : T ⊢ q ⟶ p :=
+by { have : T ⊢ p ⟶ q ⟶ p, simp,
+     exact modus_ponens this h }
+
+lemma modus_ponens_hyp {p q r: F} (hqr : T ⊢ p ⟶ q ⟶ r) (hq : T ⊢ p ⟶ q) : T ⊢ p ⟶ r :=
+by { have : T ⊢ (p ⟶ q ⟶ r) ⟶ (p ⟶ q) ⟶ p ⟶ r, simp,
+     exact modus_ponens (modus_ponens this hqr) hq }
+
+lemma imp_trans {p q r : F} : (T ⊢ p ⟶ q) → (T ⊢ q ⟶ r) → (T ⊢ p ⟶ r) := λ h₁ h₂,
+begin
+  have l₁ : T ⊢ (p ⟶ q ⟶ r) ⟶ (p ⟶ q) ⟶ (p ⟶ r), simp,  
+  have l₂ : T ⊢ (p ⟶ q ⟶ r), simp[h₂],
+  have l₃ : T ⊢ (p ⟶ q) ⟶ (p ⟶ r), from modus_ponens l₁ l₂,
+  exact modus_ponens l₃ h₁
+end
+
+@[simp] lemma dne (p : F) : T ⊢ ⁻⁻p ⟶ p :=
+begin
+  have lmm₁ : T ⊢ ⁻⁻p ⟶ (⁻⁻⁻⁻p ⟶ ⁻⁻p) ⟶ ⁻p ⟶ ⁻⁻⁻p, simp,
+  have lmm₂ : T ⊢ ⁻⁻p ⟶ ⁻⁻⁻⁻p ⟶ ⁻⁻p, simp,
+  have lmm₃ : T ⊢ ⁻⁻p ⟶ (⁻p ⟶ ⁻⁻⁻p) ⟶ ⁻⁻p ⟶ p, simp,  
+  have lmm₄ : T ⊢ ⁻⁻p ⟶ ⁻p ⟶ ⁻⁻⁻p, from modus_ponens_hyp lmm₁ lmm₂,
+  have lmm₅ : T ⊢ ⁻⁻p ⟶ ⁻⁻p ⟶ p, from modus_ponens_hyp lmm₃ lmm₄,
+  have lmm₆ : T ⊢ ⁻⁻p ⟶ ⁻⁻p, simp,
+  exact modus_ponens_hyp lmm₅ lmm₆
+end
+
+@[simp] lemma dni (p : F) : T ⊢ p ⟶ ⁻⁻p :=
+by { have : T ⊢ (⁻⁻⁻p ⟶ ⁻p) ⟶ p ⟶ ⁻⁻p, simp,
+     exact modus_ponens this (by simp) }
+
+@[simp] lemma dn_iff {p : F} : T ⊢ ⁻⁻p ↔ T ⊢ p :=
+⟨λ h, modus_ponens (show T ⊢ ⁻⁻p ⟶ p, by simp) h, λ h, modus_ponens (show T ⊢ p ⟶ ⁻⁻p, by simp) h⟩
+
+
+@[simp] lemma dn1_iff {p q : F} : (T ⊢ ⁻⁻p ⟶ q) ↔ (T ⊢ p ⟶ q) :=
+⟨imp_trans (dni _), imp_trans (dne _)⟩
+
+@[simp] lemma dn2_iff {p q : F} : (T ⊢ p ⟶ ⁻⁻q) ↔ (T ⊢ p ⟶ q) :=
+⟨λ h, imp_trans h (dne _), λ h, imp_trans h (dni _)⟩
+
+lemma explosion {p : F} (h₁ : T ⊢ p) (h₂ : T ⊢ ⁻p) {q : F} : T ⊢ q :=
+begin
+  have : T ⊢ ⁻p ⟶ ⁻q ⟶ ⁻p, simp,
+  have : T ⊢ ⁻q ⟶ ⁻p, from modus_ponens this h₂,
+  have : T ⊢ p ⟶ q, from modus_ponens (show T ⊢ (⁻q ⟶ ⁻p) ⟶ p ⟶ q, by simp) this,
+  exact modus_ponens this h₁
+end
+
+lemma explosion_hyp {p q : F} (h₁ : T ⊢ p ⟶ q) (h₂ : T ⊢ p ⟶ ⁻q) {r : F} : T ⊢ p ⟶ r :=
+begin
+  have : T ⊢ p ⟶ ⁻q ⟶ ⁻r ⟶ ⁻q, simp,
+  have : T ⊢ p ⟶ ⁻r ⟶ ⁻q, from modus_ponens_hyp this h₂,
+  have : T ⊢ p ⟶ q ⟶ r, from modus_ponens_hyp (show T ⊢ p ⟶ (⁻r ⟶ ⁻q) ⟶ q ⟶ r, by simp) this,
+  exact modus_ponens_hyp this h₁
+end
+
+@[simp] lemma hyp_bot {p : F} : T ⊢ ⊥ ⟶ p :=
+explosion_hyp (show T ⊢ (⊥ ⟶ ⊤ : F), by simp) (show T ⊢ (⊥ ⟶ ⁻⊤ : F), by simp)
+
+lemma contraposition {p q : F} : (T ⊢ ⁻p ⟶ ⁻q) ↔ (T ⊢ q ⟶ p) :=
+⟨λ h, modus_ponens (show T ⊢ (⁻p ⟶ ⁻q) ⟶ q ⟶ p, by simp) h, λ h,
+  by { refine modus_ponens (show T ⊢ (⁻⁻q ⟶ ⁻⁻p) ⟶ ⁻p ⟶ ⁻q, by simp) _,
+       have : T ⊢ ⁻⁻q ⟶ p, from imp_trans (show T ⊢ ⁻⁻q ⟶ q, by simp) h,
+       exact imp_trans this (show T ⊢ p ⟶ ⁻⁻p, by simp) }⟩
+
+lemma neg_hyp {p : F} (h : T ⊢ p ⟶ ⁻p) : T ⊢ ⁻p :=
+begin
+  have : T+{p} ⊢ ⁻(p ⟶ ⁻p),
+  { have lmm₁ : T+{p} ⊢ p, simp,
+    have lmm₂ : T+{p} ⊢ ⁻p, from modus_ponens (weakening_insert h _) lmm₁,
+    exact explosion lmm₁ lmm₂ },
+  have : T ⊢ p ⟶ ⁻(p ⟶ ⁻p), from deduction.mp this,
+  have : T ⊢ (p ⟶ ⁻p) ⟶ ⁻p, from imp_trans (dni _) (contraposition.mpr this),
+  exact modus_ponens this h
+end
+
+lemma raa {p : F} (q : F) (h₁ : T +{ p } ⊢ q) (h₂ : T +{ p } ⊢ ⁻q) : T ⊢ ⁻p :=
+neg_hyp (deduction.mp (explosion h₁ h₂))
+
+@[simp] lemma and_left (p q : F) : T ⊢ p ⊓ q ⟶ p :=
+begin
+  simp[and_def],
+  have : T+{⁻p}+{p} ⊢ ⁻q, 
+    from explosion (show T+{⁻p}+{p} ⊢ p, by simp) (show T+{⁻p}+{p} ⊢ ⁻p, by simp),
+  have : T ⊢ ⁻p ⟶ p ⟶ ⁻q, from (deduction.mp (deduction.mp this)),
+  exact imp_trans (contraposition.mpr this) (by simp)
+end
+
+@[simp] lemma and_right (p q : F) : T ⊢ p ⊓ q ⟶ q :=
+begin
+  simp[and_def],
+  have : T ⊢ ⁻q ⟶ p ⟶ ⁻q, simp,
+  have : T ⊢ ⁻(p ⟶ ⁻q) ⟶ q, from imp_trans (contraposition.mpr this) (by simp),
+  exact this
+end
+
+@[simp] lemma and {p q : F} : (T ⊢ p ⊓ q) ↔ (T ⊢ p ∧ T ⊢ q) :=
+⟨λ h, by { split,
+   { exact modus_ponens (show T ⊢ p ⊓ q ⟶ p, by simp) h },
+   { exact modus_ponens (show T ⊢ p ⊓ q ⟶ q, by simp) h } },
+ λ h, by {simp[and_def], rcases h with ⟨h₁, h₂⟩,
+   show T ⊢ ⁻(p ⟶ ⁻q),
+   have : T+{p ⟶ ⁻q} ⊢ ⁻q, from modus_ponens (insert _) (by simp[h₁]),
+   have : T ⊢ (p ⟶ ⁻q) ⟶ ⁻q, from deduction.mp this,
+   have : T ⊢ q ⟶ ⁻(p ⟶ ⁻q), from imp_trans (dni _) (contraposition.mpr this),
+   exact modus_ponens this h₂ }⟩
+
+@[simp] lemma iff {p q : F} : (T ⊢ p ⟷ q) ↔ (T ⊢ p ⟶ q ∧ T ⊢ q ⟶ p) :=
+by simp[lrarrow_def]
+
+@[simp] lemma neg_imp {p q : F} : (T ⊢ ⁻(p ⟶ q)) ↔ (T ⊢ p ⊓ ⁻q) :=
+begin
+  simp only [and_def], split; intros h,
+  { apply raa (p ⟶ q),
+    { have : T+{p ⟶ ⁻⁻q} ⊢ p ⟶ ⁻⁻q, from insert _, simp* at * },
+    { simp[h] } },
+  { apply raa (p ⟶ ⁻⁻q); simp[h] }
+end
+
+lemma or_l (p q : F) : T ⊢ p ⟶ p ⊔ q :=
+by simp[or_def]; refine deduction.mp (deduction.mp (explosion (show T +{ p } +{ ⁻p } ⊢ p, by simp) (by simp)))
+
+lemma or_r (p q : F) : T ⊢ q ⟶ p ⊔ q :=
+by simp[or_def]; refine deduction.mp (weakening h _)
+
+lemma hyp_or {p₁ p₂ q : F} : (T ⊢ p₁ ⟶ q) → (T ⊢ p₂ ⟶ q) → (T ⊢ p₁ ⊔ p₂ ⟶ q) := λ h₁ h₂,
+begin
+  simp[or_def], apply contraposition.mp, refine deduction.mp _, simp,
+  refine ⟨deduction.mpr (contraposition.mpr h₁), deduction.mpr (contraposition.mpr h₂)⟩, 
+end
+
+lemma hyp_and_left {p₁ p₂ q : F} : (T ⊢ p₁ ⟶ q) → (T ⊢ p₁ ⊓ p₂ ⟶ q) := λ h,
+begin
+  have : T+{p₁ ⊓ p₂} ⊢ p₁, { have : T+{p₁ ⊓ p₂} ⊢ p₁ ⊓ p₂, from insert _, simp* at * },
+  refine deduction.mp (modus_ponens (show T+{p₁ ⊓ p₂} ⊢ p₁ ⟶ q, by simp[h]) this)
+end
+
+lemma hyp_and_right {p₁ p₂ q : F} : (T ⊢ p₂ ⟶ q) → (T ⊢ p₁ ⊓ p₂ ⟶ q) := λ h,
+begin
+  have : T+{p₁ ⊓ p₂} ⊢ p₂, { have : T+{p₁ ⊓ p₂} ⊢ p₁ ⊓ p₂, from insert _, simp* at * },
+  refine deduction.mp (modus_ponens (show T+{p₁ ⊓ p₂} ⊢ p₂ ⟶ q, by simp[h]) this)
+end
+
+lemma axiom_and {p₁ p₂ q : F} : T +{ p₁ ⊓ p₂ } ⊢ q ↔ T +{ p₁ } +{ p₂ } ⊢ q :=
+⟨λ h,
+ by { have lmm₁ : T+{p₁}+{p₂} ⊢ p₁ ⊓ p₂, by simp,
+      have lmm₂ : T+{p₁}+{p₂} ⊢ p₁ ⊓ p₂ ⟶ q, simp[deduction.mp h],
+      exact modus_ponens lmm₂ lmm₁ },
+ λ h,
+ by { have lmm₁ : T+{p₁ ⊓ p₂} ⊢ p₁ ⟶ p₂ ⟶ q, simp[deduction.mp (deduction.mp h)],
+      have lmm₂ : T+{p₁ ⊓ p₂} ⊢ p₁ ⊓ p₂, from insert _, simp at lmm₂,
+      exact modus_ponens (modus_ponens lmm₁ lmm₂.1) lmm₂.2 } ⟩
+
+end classical_logic
+
